Alexander Hatle
![[Pasted image 20241025154944.png|700]]
![[Pasted image 20241025154833.png|500]]
![[Pasted image 20241025153439.png|700]]
$$\Psi (I_{1},I_{4},J)=c_{1}(I_{1}-3)+2\frac{k_{1}}{k_{2}}(\exp(k_{2}(I_{4}-1)^{2})-1)-p(J-1)$$

$$\begin{aligned}
\mathbf S&= 2\frac{\partial \Psi }{\partial \mathbf C}\\
&= 2\left(\frac{\partial \Psi }{\partial I_{1}} \frac{\partial I_{1}}{\partial \mathbf C}+\frac{\partial \Psi }{\partial I_{4}} \frac{\partial I_{4}}{\partial \mathbf C}+\frac{\partial \Psi }{\partial J} \frac{\partial J}{\partial \mathbf C}\right).
\end{aligned}$$
We are already given $\frac{\partial I_{1}}{\partial \mathbf C},\frac{\partial J}{\partial \mathbf C}$, so let's calculate $\frac{\partial I_{4}}{\partial \mathbf C}$:
$$\begin{aligned}
I_{4}&= a_{0i}C_{ij}a_{0j}\\
\frac{\partial I_{4}}{\partial C_{kl}}&= a_{0i}\frac{\partial C_{ij}}{\partial C_{kl}}a_{0j}\\
&= a_{0i}\delta _{ik}\delta _{jl}a_{0j}\\
&= a_{0k} a_{0l}\\
&= \mathbf a_{0}\otimes \mathbf a_{0}.
\end{aligned}$$
Since the material is incompressible, $J=\det F=\lambda _{1}\lambda _{2}=1$, and $\lambda _{2}=\frac{1}{\lambda _{1}}$. Substituting:
$$\begin{aligned}
\mathbf S&= 2\left(\frac{\partial \Psi }{\partial I_{1}} \mathbf I+\frac{\partial \Psi }{\partial I_{4}} \mathbf a_{0}\otimes \mathbf a_{0}+\frac{\partial \Psi }{\partial J}\frac{1}{2}J \mathbf C^{-1}\right)\\
&= 2c_{1}\mathbf I+\left[8k_{1}(I_{4}-1)\cdot \exp(k_{2}(I_{4}-1)^{2}) \right]a_{0}\otimes a_{0}-pC^{-1}.
\end{aligned}$$
The stress matrix is
$$\begin{aligned}
\sigma &= \frac{1}{J}\mathbf F \mathbf S \mathbf F^{T}\\
&= \mathbf F \left(2c_{1}\mathbf I+\left[8k_{1}(I_{4}-1)\cdot \exp((k_{2}(I_{4}-1)^{2})) \right]\mathbf a_{0}\otimes \mathbf a_{0}-pC^{-1} \right)\mathbf F^{T}\\
&= 2c_{1}\mathbf b+\left[8k_{1}(I_{4}-1)\cdot \exp((k_{2}(I_{4}-1)^{2})) \right]\mathbf F \mathbf a_{0}\otimes \mathbf a_{0} \mathbf F^{T}-p \mathbf I\\
&=  2c_{1}\mathbf b+\left[8k_{1}(I_{4}-1)\cdot \exp(k_{2}(I_{4}-1)^{2}) \right]\mathbf a \otimes \mathbf a-p \mathbf I.
\end{aligned}\tag{1}$$
Setting up expressions for $\mathbf F, \mathbf b,\mathbf a \otimes \mathbf a$:
$$\begin{aligned}
\mathbf F&= \begin{bmatrix}\lambda _{1} & 0\\
0 & \lambda _{2}\end{bmatrix}\\
&= \begin{bmatrix}\lambda _{1} & 0\\
0 & \frac{1}{\lambda _{1}}\end{bmatrix}\\
\mathbf b &= \mathbf F \mathbf F^{T}\\
&= \begin{bmatrix}\lambda _{1}^{2} & 0\\
0 & \frac{1}{\lambda _{1}^{2}}\end{bmatrix}\\
\mathbf a \otimes \mathbf a&= \mathbf F \mathbf a_{0}\otimes \mathbf F \mathbf a_{0}\\
&= \begin{bmatrix}\lambda _{1} & 0\\
0 & \frac{1}{\lambda _{1}}\end{bmatrix}\begin{bmatrix}1\\
0\end{bmatrix}\otimes \begin{bmatrix}\lambda _{1} & 0\\
0 & \frac{1}{\lambda _{1}}\end{bmatrix}\begin{bmatrix}1\\
0\end{bmatrix}\\
&= \begin{bmatrix}\lambda _{1} \\
0\end{bmatrix}\otimes \begin{bmatrix}\lambda _{1}\\
0\end{bmatrix}\\
&= \begin{bmatrix}\lambda _{1}^{2} & 0\\
0 & 0\end{bmatrix}.
\end{aligned}$$
Substituting into (1):
$$\begin{aligned}
\begin{bmatrix}\sigma _{1} & 0\\
0 & \sigma _{2}\end{bmatrix}&= 2c_{1}\begin{bmatrix}\lambda _{1} ^{2} & 0\\
0 & \frac{1}{\lambda _{1}^{2}}\end{bmatrix}+\left[8k_{1}(I_{4}-1)\cdot \exp(k_{2}(I_{4}-1)^{2}) \right]\begin{bmatrix}\lambda _{1}^{2} & 0\\
0 & 0\end{bmatrix}-p\begin{bmatrix}1 & 0\\
0 & 1\end{bmatrix}.
\end{aligned}$$
Since we are loading the bar uniaxially, we set $\sigma _{2}=0$ to get
$$\begin{aligned}
0&= 2c_{1}\frac{1}{\lambda _{1}^{2}}-p\\
p&= \frac{2c_{1}}{\lambda _{1}^{2}}.
\end{aligned}$$
Then, the equation for $\sigma _{1}$ is
$$\begin{aligned}
\sigma _{1}&= 2c_{1}\lambda _{1}^{2}+8k_{1}(I_{4}-1)\cdot \exp(k_{2}(I_{4}-1)^{2})\lambda _{1}^{2}-\frac{2c_{1}}{\lambda _{1}^{2}}\\
&= \left[2c_{1}+8k_{1}(I_{4}-1)\exp(k_{2}(I_{4}-1)^{2}) \right]\lambda _{1}^{2}- \frac{2c_{1}}{\lambda _{1}^{2}}.
\end{aligned}$$
We find $I_{4}$ as
$$\begin{aligned}
I_{4}&= \mathbf a_{0}\mathbf C \mathbf a_{0}\\
&= \mathbf a_{0}\mathbf F^{T}\mathbf F \mathbf a_{0}\\
&= \begin{bmatrix}1\\
0\end{bmatrix}\begin{bmatrix}\lambda _{1} & 0\\
0 & \frac{1}{\lambda _{1}}\end{bmatrix}\begin{bmatrix}\lambda _{1} & 0\\
0 & \frac{1}{\lambda _{1}}\end{bmatrix}\begin{bmatrix}1\\
0\end{bmatrix}\\
&= \lambda _{1}^{2}
\end{aligned}$$
Since $\sigma _{1}= \frac{P}{A_{0}}$, we can set up the expression for $P$:
$$P=\left[2c_{1}+8k_{1}(\lambda _{1}^{2}-1)\exp(k_{2}(\lambda _{1}^{2}-1)^{2}) \right]A_{0}\lambda _{1}^{2}- \frac{2c_{1}A_{0}}{\lambda _{1}^{2}}.$$
![[Pasted image 20241025154856.png|700]]


![[Pasted image 20241025154922.png|700]]
![[Pasted image 20241025155005.png|500]]

![[Pasted image 20241025155029.png|700]]
![[Pasted image 20241025155044.png|700]]
![[Pasted image 20241025155058.png|700]]
Very similar to exercise 5.
$$\Psi  (I_{1},J,I_{4_{1}},I_{4_{2}})=\frac{c}{2}(I_{1}-3)+\frac{k_{1}}{2k_{2}}\sum_{i=1,2}\left(\exp[k_{2}(I_{4_{i}}-1)^{2}]-1 \right)+p(J-1)$$
$$\mathbf \sigma =\frac{1}{J} \mathbf F \mathbf S \mathbf F^{T}$$
Let's first find $\mathbf S$:
$$\begin{aligned}
\mathbf S&=  2 \frac{\partial \Psi }{\partial C}\\
S_{ij}&=2 \frac{\partial \Psi }{\partial C_{ij}} \\
&= 2\left(\frac{\partial \Psi }{\partial J}\frac{\partial J}{\partial C_{ij}}+\frac{\partial \Psi }{\partial I_{1}}\frac{\partial I_{1}}{\partial C_{ij}}+\frac{\partial \Psi }{\partial I_{4_{1}}}\frac{\partial I_{4_{1}}}{\partial C_{ij}} +\frac{\partial \Psi }{\partial I_{4_{2}}}\frac{\partial I_{4_{2}}}{\partial C_{ij}} \right)
\end{aligned}$$
The terms are
$$\begin{aligned}
\frac{\partial \Psi }{\partial J}&= p\\
\frac{\partial J}{\partial C_{ij}}&= \frac{1}{2}J \mathbf C^{-1}\\
\frac{\partial \Psi }{\partial I_{1}}&= \frac{c}{2}\\
	\frac{\partial I_{1}}{\partial C_{ij}}&= \mathbf 1\\
\frac{\partial \Psi }{\partial I_{4_{1}}}&= k_{1}(I_{4_{1}}-1)\exp(k_{2}(I_{4_{1}}-1)^{2}-1)\\
\frac{\partial I_{4_{1}}}{\partial C_{ij}}&=  m_{0k}\frac{\partial C_{kl}}{\partial C_{ij}} m_{0l}\\
&= m_{0k}\delta _{ik} \delta _{jl}m_{0l}\\
&= m_{0i}m_{0j}\\
&= \mathbf m_{0}\otimes \mathbf m_{0}\\
\frac{\partial \Psi }{\partial I_{4_{2}}}&= k_{1}(I_{4_{2}}-1)\exp(k_{2}(I_{4_{2}}-1)^{2}-1)\\
\frac{\partial I_{4_{1}}}{\partial C_{ij}}&=   \mathbf m_{0}'\otimes \mathbf m_{0}'
\end{aligned}$$
Substituting into the equation for the second Piola-Kirchoff stress tensor:
$$\begin{aligned}
\mathbf S&= 2 \left(\frac{p}{2}J \mathbf C^{-1}+ \frac{c}{2}\mathbf I+  k_{1}(I_{4_{1}}-1)\exp(k_{2}(I_{4_{1}}-1)^{2}-1) \mathbf m_{0}\otimes \mathbf m_{0}+ k_{1}(I_{4_{2}}-1)\exp(k_{2}(I_{4_{2}}-1)^{2}-1) \mathbf m_{0}'\otimes \mathbf m_{0}'\right)\\
&= pJ \mathbf C^{-1}+ c\mathbf I+  2k_{1}(I_{4_{1}}-1)\exp(k_{2}(I_{4_{1}}-1)^{2}-1) \mathbf m_{0}\otimes \mathbf m_{0}+ 2k_{1}(I_{4_{2}}-1)\exp(k_{2}(I_{4_{2}}-1)^{2}-1) \mathbf m_{0}'\otimes \mathbf m_{0}',
\end{aligned}$$
allowing us to set the expression for the Cauchy stress tensor as
$$\begin{aligned}
\mathbf \sigma &= \frac{1}{J} \mathbf F\left( pJ \mathbf C^{-1}+ c\mathbf I+  2k_{1}(I_{4_{1}}-1)\exp(k_{2}(I_{4_{1}}-1)^{2}-1) \mathbf m_{0}\otimes \mathbf m_{0}+ 2k_{1}(I_{4_{2}}-1)\exp(k_{2}(I_{4_{2}}-1)^{2}-1) \mathbf m_{0}'\otimes \mathbf m_{0}'\right) \mathbf F^{T}\\
&= \frac{1}{J}\left(pJ \mathbf F (\mathbf F^{T}\mathbf F)^{-1}\mathbf F^{T}+ c\mathbf F \mathbf F^{T}+  2k_{1}(I_{4_{1}}-1)\exp(k_{2}(I_{4_{1}}-1)^{2}-1) \mathbf F\mathbf m_{0}\otimes \mathbf m_{0}\mathbf F^{T}+ 2k_{1}(I_{4_{2}}-1)\exp(k_{2}(I_{4_{2}}-1)^{2}-1) \mathbf F\mathbf m_{0}'\otimes \mathbf m_{0}'\mathbf F^{T} \right)\\
&= \frac{1}{J}\left(pJ \mathbf I+ c\mathbf b+  2k_{1}(I_{4_{1}}-1)\exp(k_{2}(I_{4_{1}}-1)^{2}-1) \mathbf m\otimes \mathbf m\mathbf + 2k_{1}(I_{4_{2}}-1)\exp(k_{2}(I_{4_{2}}-1)^{2}-1) \mathbf m'\otimes \mathbf m' \right).
\end{aligned}$$
Due to incompressibility, we have that $J=\det F= \lambda _{1}\lambda _{2}\lambda _{3}=1$ so
$$\mathbf \sigma =p \mathbf I+ c\mathbf b+  2k_{1}(I_{4_{1}}-1)\exp(k_{2}(I_{4_{1}}-1)^{2}-1) \mathbf m\otimes \mathbf m\mathbf + 2k_{1}(I_{4_{2}}-1)\exp(k_{2}(I_{4_{2}}-1)^{2}-1) \mathbf m'\otimes \mathbf m' ,\tag{2}$$
and since $\lambda _{3}=\frac{1}{\lambda _{1}\lambda _{2}}$, the deformation gradient tensor is
$$\begin{aligned}
\mathbf F&= \begin{bmatrix}\lambda _{1} & 0 & 0 \\ 0 & \lambda _{2} & 0 \\ 0 & 0 & \lambda _{3}\end{bmatrix}\\
&= \begin{bmatrix}\lambda _{1} & 0 & 0 \\ 0 & \lambda _{2} & 0 \\ 0 & 0 & \frac{1}{(\lambda _{1}\lambda _{2})^{2}}\end{bmatrix}.
\end{aligned}$$
The left Cauchy-Green tensor is
$$\begin{aligned}
\mathbf b &=  \mathbf F \mathbf F^{T}\\
&= \begin{bmatrix}\lambda _{1}^{2} & 0 & 0\\
0 & \lambda _{2}^{2} & 0\\
0 & 0 & \frac{1}{(\lambda _{1}\lambda _{2})^{2}}\end{bmatrix}.
\end{aligned}$$
The mean fiber directions are described by
$$\begin{aligned}
\mathbf m_{0}&= \begin{bmatrix}\cos \theta _{1}\\
\sin \theta _{1}\\
0\end{bmatrix}\\
\mathbf m_{0}'&= \begin{bmatrix}\cos \theta _{2}\\
-\sin \theta _{2}\\
0\end{bmatrix}.
\end{aligned}$$
Assuming $\theta _{1}=\theta _{2}=\theta$, we can find the deformed fiber directions $\mathbf m, \mathbf m'$:
$$\begin{aligned}
\mathbf m&= \mathbf F \mathbf m_{0}\\
&= \begin{bmatrix}\lambda _{1} & 0 & 0 \\ 0 & \lambda _{2} & 0 \\ 0 & 0 & \frac{1}{(\lambda _{1}\lambda _{2})^{2}}\end{bmatrix}\begin{bmatrix}\cos \theta \\
\sin \theta \\
0\end{bmatrix}\\
&= \begin{bmatrix}\lambda _{1}\cos \theta \\
\lambda _{2}\sin \theta \\
0\end{bmatrix}\\
\mathbf m'&= \begin{bmatrix}\lambda _{1}\cos \theta \\
-\lambda _{2}\sin \theta \\
0\end{bmatrix},
\end{aligned}$$
and the dyadic products become
$$\begin{aligned}
\mathbf m \otimes \mathbf m&= \begin{bmatrix}\lambda _{1}\cos \theta \\
\lambda _{2}\sin \theta \\
0\end{bmatrix} \otimes \begin{bmatrix}\lambda _{1}\cos \theta \\
\lambda _{2}\sin \theta \\
0\end{bmatrix}\\
&= \begin{bmatrix}\lambda _{1}^{2}\cos ^{2}\theta  & \lambda _{1}\lambda _{2}\sin \theta \cos \theta  & 0\\
\lambda _{1}\lambda _{2}\sin \theta \cos \theta  & \lambda _{2}\sin ^{2}\theta  & 0\\
0 & 0 & 0\end{bmatrix}\\
\mathbf m' \otimes \mathbf m'&= \begin{bmatrix}\lambda _{1}\cos \theta \\
-\lambda _{2}\sin \theta \\
0\end{bmatrix} \otimes \begin{bmatrix}\lambda _{1}\cos \theta \\
-\lambda _{2}\sin \theta \\
0\end{bmatrix}\\
&= \begin{bmatrix}\lambda _{1}^{2}\cos ^{2}\theta  & -\lambda _{1}\lambda _{2}\sin \theta \cos \theta  & 0\\
-\lambda _{1}\lambda _{2}\sin \theta \cos \theta  & \lambda _{2}\sin ^{2}\theta  & 0\\
0 & 0 & 0\end{bmatrix}.
\end{aligned}$$

Substituting all these values into (2):
$$\begin{aligned}
\mathbf \sigma &= p \mathbf I+ c\mathbf b+  2k_{1}(I_{4_{1}}-1)\exp(k_{2}(I_{4_{1}}-1)^{2}-1) \mathbf m\otimes \mathbf m\mathbf + 2k_{1}(I_{4_{2}}-1)\exp(k_{2}(I_{4_{2}}-1)^{2}-1) \mathbf m'\otimes \mathbf m' \\
\begin{bmatrix}\sigma _{11} & \sigma _{12} & \sigma _{13}\\
\sigma _{21} & \sigma _{22} & \sigma _{23}\\
\sigma _{31} & \sigma _{32} & \sigma _{33}\end{bmatrix}&= p\begin{bmatrix}1 & 0 & 0\\
0 & 1 & 0\\
0 & 0 & 1\end{bmatrix}+c\begin{bmatrix}\lambda _{1}^{2} & 0 & 0\\
0 & \lambda _{2}^{2} & 0\\
0 & 0 & \frac{1}{(\lambda _{1}\lambda _{2})^{2}}\end{bmatrix}\\
&+2k_{1}(I_{4_{1}}-1)\exp(k_{2}(I_{4_{1}}-1)^{2}-1)\begin{bmatrix}\lambda _{1}^{2}\cos ^{2}\theta  & \lambda _{1}\lambda _{2}\sin \theta \cos \theta  & 0\\
\lambda _{1}\lambda _{2}\sin \theta \cos \theta  & \lambda _{2}\sin ^{2}\theta  & 0\\
0 & 0 & 0\end{bmatrix}\\
&+2k_{1}(I_{4_{2}}-1)\exp(k_{2}(I_{4_{2}}-1)^{2}-1)
\begin{bmatrix}\lambda _{1}^{2}\cos ^{2}\theta  & -\lambda _{1}\lambda _{2}\sin \theta \cos \theta  & 0\\
-\lambda _{1}\lambda _{2}\sin \theta \cos \theta  & \lambda _{2}\sin ^{2}\theta  & 0\\
0 & 0 & 0\end{bmatrix}

\end{aligned}$$
Calculating $I_{4_{1}},I_{4_{2}}$:
$$\begin{aligned}
I_{4_{1}}&= \mathbf m_{0}\cdot \mathbf C \cdot \mathbf m_{0}\\
&= \mathbf m_{0}\cdot \mathbf F ^{T}\mathbf F \cdot \mathbf m_{0}\\
&= \begin{bmatrix}\lambda _{1}\cos \theta \\
\lambda _{2}\sin \theta \\
0\end{bmatrix}\cdot \begin{bmatrix}\lambda _{1}\cos \theta \\
\lambda _{2}\sin \theta \\
0\end{bmatrix}\\
&= \lambda _{1}\cos ^{2}\theta +\lambda _{2}\sin ^{2}\theta, \\
I_{4_{2}}&= \mathbf m_{0}'\cdot \mathbf C \cdot \mathbf m_{0}'\\
&= \begin{bmatrix}\lambda _{1}\cos \theta \\
-\lambda _{2}\sin \theta \\
0\end{bmatrix}\cdot \begin{bmatrix}\lambda _{1}\cos \theta \\
-\lambda _{2}\sin \theta \\
0\end{bmatrix}\\
&= \lambda _{1}\cos ^{2}\theta +\lambda _{2}\sin ^{2}\theta.
\end{aligned}$$
Let $I_{4}=I_{4_{1}}=I_{4_{2}}$, so $(2)$ becomes
$$\begin{aligned}
\begin{bmatrix}\sigma _{11} & \sigma _{12} & \sigma _{13}\\
\sigma _{21} & \sigma _{22} & \sigma _{23}\\
\sigma _{31} & \sigma _{32} & \sigma _{33}\end{bmatrix}&=\begin{bmatrix}p+c\lambda _{1}^{2} & 0 & 0\\
0 & p+c\lambda _{2}^{2} & 0\\
0 & 0 & p+\frac{c}{(\lambda _{1}\lambda _{2})^{2}}\end{bmatrix}
+4k_{1}(I_{4}-1)\exp(k_{2}(I_{4}-1)^{2}-1)
\begin{bmatrix}\lambda _{1}^{2}\cos ^{2}\theta  & 0  & 0\\
0  & \lambda _{2}\sin ^{2}\theta  & 0\\
0 & 0 & 0\end{bmatrix}.
\end{aligned}$$

Due to plane stress conditions, we set $\sigma _{33}=0$ in order to determine $p$:
$$\begin{aligned}
\sigma _{33}&= 0\\
p&= -\frac{c}{(\lambda _{1}\lambda _{2})^{2}},
\end{aligned}$$
giving us the final expressions for $\sigma _{11}$ and $\sigma _{22}$
$$\begin{aligned}
\sigma _{11} &=-\frac{c}{(\lambda _{1}\lambda _{2})^{2}}+c\lambda _{1}^{2}
+4k_{1}(I_{4}-1)\exp(k_{2}(I_{4}-1)^{2}-1)\lambda _{1}^{2}\cos ^{2}\theta \\
\sigma _{22} &=-\frac{c}{(\lambda _{1}\lambda _{2})^{2}}+c\lambda _{2}^{2}
+4k_{1}(I_{4}-1)\exp(k_{2}(I_{4}-1)^{2}-1)\lambda _{2}^{2}\sin ^{2}\theta.
\end{aligned}$$


![[Pasted image 20241025155118.png|700]]
$$\Psi  (I_{1},J,I_{4_{1}},I_{4_{2}})=\frac{c}{2}(I_{1}-3)+\frac{k_{1}}{2k_{2}}\sum_{i=1,2}\left(\exp[k_{2}(\kappa I_{1}+(1-3\kappa )I_{4_{i}}-1)^{2}]-1 \right)+p(J-1)$$
The second Piola-Kirchoff stress is still
$$\begin{aligned}
\mathbf S&= 2\left(\frac{\partial \Psi }{\partial J}\frac{\partial J}{\partial \mathbf C}+\frac{\partial \Psi }{\partial I_{1}}\frac{\partial I_{1}}{\partial \mathbf C}+\frac{\partial \Psi }{\partial I_{4_{1}}}\frac{\partial I_{4_{1}}}{\partial \mathbf C} +\frac{\partial \Psi }{\partial I_{4_{2}}}\frac{\partial I_{4_{2}}}{\partial \mathbf C} \right)
\end{aligned}$$
The following terms are the same as before:
$$\begin{aligned}
\frac{\partial \Psi }{\partial J}&= p\\
\frac{\partial J}{\partial \mathbf C}&= \frac{1}{2}J \mathbf C^{-1}\\
\frac{\partial I_{1}}{\partial \mathbf C}&= \mathbf 1\\
\frac{\partial I_{4_{1}}}{\partial \mathbf C}&=  m_{0k}\frac{\partial C_{kl}}{\partial C_{ij}} m_{0l}\\
&= m_{0k}\delta _{ik} \delta _{jl}m_{0l}\\
&= m_{0i}m_{0j}\\
&= \mathbf m_{0}\otimes \mathbf m_{0}\\
\frac{\partial I_{4_{1}}}{\partial \mathbf C}&=   \mathbf m_{0}'\otimes \mathbf m_{0}'.
\end{aligned}$$
So we need to find $\frac{\partial \Psi }{\partial I_{1}},\frac{\partial \Psi }{\partial I_{4_{1}}}$ and $\frac{\partial \Psi }{\partial I_{4_{2}}}$. For simplicity of notation, denote
$$f(I_{1},I_{4_{i}})=\kappa I_{1}+(1-3\kappa )I_{4_{i}}-1,$$
such that $\Psi$ can be written as 
$$\Psi  (I_{1},J,I_{4_{1}},I_{4_{2}})=\frac{c}{2}(I_{1}-3)+\frac{k_{1}}{2k_{2}}\sum_{i=1,2}\left(\exp[k_{2}(f(I_{1},I_{4_{i}}))^{2}]-1 \right)+p(J-1).$$
Then, 
$$\begin{aligned}
\frac{\partial \Psi }{\partial I_{1}}&= \frac{c}{2}+\sum_{i=1,2}^{}\frac{k_{1}}{2k_{2}}\cdot 2k_{2}f(I_{1},I_{4_{i}})\frac{\partial f(I_{1},I_{4_{i}})}{\partial I_{1}}\exp[k_{2}(f(I_{1},I_{4_{i}})^{2})-1]\\
&= \frac{c}{2}+\sum_{i=1,2}^{}k_{1}\kappa f(I_{1},I_{4_{i}})\exp[k_{2}(f(I_{1},I_{4_{i}})^{2})-1]\\
\frac{\partial \Psi }{\partial I_{4_{i}}}&= \frac{k_{1}}{2k_{2}}2k_{2}f(I_{1},I_{4_{i}})\frac{\partial f(I_{1},I_{4_{i}})}{\partial I_{4_{i}}}\exp[k_{2}(f(I_{1},I_{4_{i}})^{2})-1]\\
&= k_{1}(1-3\kappa )f(I_{1},I_{4_{i}})\exp[k_{2}(f(I_{1},I_{4_{i}})^{2})-1].
\end{aligned}$$
The Cauchy stress tensor can now be calculated as
$$\begin{aligned}
\mathbf \sigma &= \frac{1}{J}\mathbf F\mathbf S \mathbf F^{T}\\
&= \frac{2}{J} \mathbf F\left(\frac{\partial \Psi }{\partial J}\frac{\partial J}{\partial \mathbf C}+\frac{\partial \Psi }{\partial I_{1}}\frac{\partial I_{1}}{\partial \mathbf C}+\frac{\partial \Psi }{\partial I_{4_{1}}}\frac{\partial I_{4_{1}}}{\partial \mathbf C} +\frac{\partial \Psi }{\partial I_{4_{2}}}\frac{\partial I_{4_{2}}}{\partial \mathbf C} \right)\mathbf F^{T}\\
&= \frac{1}{J}\left(2\mathbf F\frac{\partial \Psi }{\partial J}\frac{\partial J}{\partial \mathbf C}\mathbf F^{T}+2\mathbf F\frac{\partial \Psi }{\partial I_{1}}\frac{\partial I_{1}}{\partial \mathbf C}\mathbf F^{T}+2\mathbf F\frac{\partial \Psi }{\partial I_{4_{1}}}\frac{\partial I_{4_{1}}}{\partial \mathbf C}\mathbf F^{T} +2\mathbf F\frac{\partial \Psi }{\partial I_{4_{2}}}\frac{\partial I_{4_{2}}}{\partial \mathbf C}\mathbf F^{T} \right)
\end{aligned}$$
Let's calculate each term on its own:
$$\begin{aligned}
2\mathbf F\frac{\partial \Psi }{\partial J}\frac{\partial J}{\partial \mathbf C}\mathbf F^{T}&= 2\mathbf Fp \frac{1}{2}J \mathbf C^{-1}\mathbf F^{T}\\
&= pJ \mathbf 1\\
2\mathbf F\frac{\partial \Psi }{\partial I_{1}}\frac{\partial I_{1}}{\partial \mathbf C}\mathbf F^{T}&= 2\mathbf F \left(\frac{c}{2}+\sum_{i=1,2}^{}k_{1}\kappa f(I_{1},I_{4_{i}})\exp[k_{2}(f(I_{1},I_{4_{i}})^{2})-1] \right) \mathbf 1\mathbf F^{T}\\
&= \left(c+2k_{1}\kappa \sum_{i=1,2}^{}f(I_{1},I_{4_{i}})\exp[k_{2}(f(I_{1},I_{4_{i}})^{2})-1] \right) \mathbf b\\
2\mathbf F\frac{\partial \Psi }{\partial I_{4_{1}}}\frac{\partial I_{4_{1}}}{\partial \mathbf C}\mathbf F^{T}&= 2 \mathbf F k_{1}(1-3\kappa )f(I_{1},I_{4_{1}})\exp[k_{2}(f(I_{1},I_{4_{1}})^{2})-1] \mathbf m_{0}\otimes \mathbf m_{0} \mathbf F^{T}\\
&= 2k_{1}(1-3\kappa )f(I_{1},I_{4_{1}})\exp[k_{2}(f(I_{1},I_{4_{1}})^{2})-1] \mathbf m \otimes \mathbf m\\
2\mathbf F\frac{\partial \Psi }{\partial I_{4_{2}}}\frac{\partial I_{4_{2}}}{\partial \mathbf C}\mathbf F^{T}&= 2k_{1}(1-3\kappa )f(I_{1},I_{4_{2}})\exp[k_{2}(f(I_{1},I_{4_{2}})^{2})-1] \mathbf m' \otimes \mathbf m'.
\end{aligned}$$
To simplify the notation further, denote
$$g(i)=2k_{1}f(I_{1},I_{4_{i}})\exp[k_{2}(f(I_{1},I_{4_{i}})^{2})-1].$$
This, with the incompressibility gives us
$$\mathbf \sigma =p \mathbf 1+ \left(c+\kappa g(1)+\kappa g(2) \right)\mathbf b+(1-3\kappa )g(1) \mathbf m \otimes \mathbf m+(1-3\kappa )g(2) \mathbf m'\otimes \mathbf m'.$$
$\mathbf b, \mathbf m\otimes \mathbf m,$ and $\mathbf m'\otimes \mathbf m'$ are the same as previously. Substituting these:

$$\begin{aligned}
\begin{bmatrix}\sigma _{11} & \sigma _{12} & \sigma _{13}\\
\sigma _{21} & \sigma _{22} & \sigma _{23}\\
\sigma _{31} & \sigma _{32} & \sigma _{33}\end{bmatrix}&= p\begin{bmatrix}1 & 0 & 0\\
0 & 1 & 0\\
0 & 0 & 1\end{bmatrix}+(c+\kappa g(1)+\kappa g(2))\begin{bmatrix}\lambda _{1}^{2} & 0 & 0\\
0 & \lambda _{2}^{2} & 0\\
0 & 0 & \frac{1}{(\lambda _{1}\lambda _{2})^{2}}\end{bmatrix}\\
&+ (1-3\kappa )g(1)\begin{bmatrix}\lambda _{1}^{2}\cos ^{2}\theta  & \lambda _{1}\lambda _{2}\sin \theta \cos \theta  & 0\\
\lambda _{1}\lambda _{2}\sin \theta \cos \theta  & \lambda _{2}\sin ^{2}\theta  & 0\\
0 & 0 & 0\end{bmatrix}\\
&+ (1-3\kappa )g(2)\begin{bmatrix}\lambda _{1}^{2}\cos ^{2}\theta  & -\lambda _{1}\lambda _{2}\sin \theta \cos \theta  & 0\\
-\lambda _{1}\lambda _{2}\sin \theta \cos \theta  & \lambda _{2}\sin ^{2}\theta  & 0\\
0 & 0 & 0\end{bmatrix}.
\end{aligned}$$

Setting $\sigma _{33}=0$ gives
$$\begin{aligned}
\sigma _{33}&= 0\\
p+(c+\kappa g(1)+\kappa g(2))\frac{1}{(\lambda _{1}\lambda _{2})^{2}}&= 0\\
p &= -\frac{c+\kappa g(1)+\kappa g(2)}{(\lambda _{1}\lambda _{2})^{2}}.
\end{aligned}$$
Finally, the equations for $\sigma _{11}$ and $\sigma _{22}$ are
$$\begin{aligned}
\sigma _{11}&= (c+\kappa g(1)+\kappa g(2)) \left(\lambda _{1}^{2}-\frac{1}{(\lambda _{1}\lambda _{2})^{2}} \right)+(1-3\kappa )(g(1)+g(2))\lambda _{1}^{2}\cos ^{2}\theta \\
\sigma _{22}&= (c+\kappa g(1)+\kappa g(2)) \left(\lambda _{2}^{2}-\frac{1}{(\lambda _{1}\lambda _{2})^{2}} \right)+(1-3\kappa )(g(1)+g(2))\lambda _{2}^{2}\sin ^{2}\theta 
\end{aligned}$$
As before,
$$I_{4}=I_{4_{1}}=I_{4_{2}}=\lambda _{1}\cos ^{2}\theta +\lambda _{2}\sin ^{2}\theta, $$
and
$$\begin{aligned}
I_{1}&= \text{tr}\mathbf C\\
&= \text{tr }\begin{bmatrix}\lambda _{1}^{2} & 0 & 0\\
0 & \lambda _{2}^{2} & 0\\
0 & 0 & \frac{1}{(\lambda _{1}\lambda _{2})^{2}}\end{bmatrix}\\
&= \lambda _{1}^{2}+\lambda _{2}^{2}+\frac{1}{(\lambda _{1}\lambda _{2})^{2}}.
\end{aligned}$$
Then, because $I_{4_{1}}=I_{4_{2}}$,
$$\begin{aligned}
g(1)&= 2k_{1}f(I_{1},I_{4_{1}})\exp[k_{2}(f(I_{1},I_{4_{1}})^{2})-1]\\
&= 2k_{1}(\kappa I_{1}+(1-3\kappa )I_{4_{1}}-1)\exp[k_{2}(\kappa I_{1}+(1-3\kappa )I_{4_{1}}-1)^{2}-1]\\
&= g(2)\\
&= :g,
\end{aligned}$$
which simplifies the expressions to
$$\begin{aligned}
\sigma _{11}&= (c+2\kappa g) \left(\lambda _{1}^{2}-\frac{1}{(\lambda _{1}\lambda _{2})^{2}} \right)+2g(1-3\kappa )\lambda _{1}^{2}\cos ^{2}\theta \\
\sigma _{22}&= (c+2\kappa g) \left(\lambda _{2}^{2}-\frac{1}{(\lambda _{1}\lambda _{2})^{2}} \right)+2g(1-3\kappa )\lambda _{2}^{2}\sin ^{2}\theta .
\end{aligned}$$


![[Pasted image 20241025155145.png|700]]
$$\Psi (I_{1},J,I_{4_{1}}^{*},I_{4_{2}}^{*})=\frac{c}{2}(I_{1}-3)+\frac{k_{1}}{2k_{2}}\sum_{i=1,2}^{}\left(\expÂ \left[k_{2}(I_{4_{i}}^{*}-1)^{2} \right] -1\right)+p(J-1)$$
The second Piola-Kirchoff stress is still
$$
\mathbf S= 2\left(\frac{\partial \Psi }{\partial J}\frac{\partial J}{\partial \mathbf C}+\frac{\partial \Psi }{\partial I_{1}}\frac{\partial I_{1}}{\partial \mathbf C}+\frac{\partial \Psi }{\partial I^{*}_{4_{1}}}\frac{\partial I^{*}_{4_{1}}}{\partial \mathbf C} +\frac{\partial \Psi }{\partial I^{*}_{4_{2}}}\frac{\partial I^{*}_{4_{2}}}{\partial \mathbf C} \right),
$$
and the Cauchy Stress tensor is
$$\mathbf \sigma =\frac{1}{J}\left(2\mathbf F\frac{\partial \Psi }{\partial J}\frac{\partial J}{\partial \mathbf C}\mathbf F^{T}+2\mathbf F\frac{\partial \Psi }{\partial I_{1}}\frac{\partial I_{1}}{\partial \mathbf C}\mathbf F^{T}+2\mathbf F\frac{\partial \Psi }{\partial I_{4_{1}}^{*}}\frac{\partial I_{4_{1}}^{*}}{\partial \mathbf C}\mathbf F^{T} +2\mathbf F\frac{\partial \Psi }{\partial I_{4_{2}}^{*}}\frac{\partial I_{4_{2}}^{*}}{\partial \mathbf C}\mathbf F^{T} \right)$$
We need to calculate $\frac{\partial \Psi }{\partial I_{1}},\frac{\partial \Psi }{\partial I_{4_{1}}^{*}}$ and $\frac{\partial \Psi }{\partial I_{4_{2}}^{*}}$:
$$\begin{aligned}
\frac{\partial \Psi }{\partial I_{1}}&= \frac{c}{2}+\sum_{i=1,2}^{}\frac{k_{1}}{2k_{2}}\cdot 2k_{2}(I_{4_{i}}^{*}-1) \frac{\partial I_{4_{i}}^{*}}{\partial I_{1}}\exp[k_{2}(I_{4_{i}}^{*}-1)^{2})-1]\\
&= \frac{c}{2}+\sum_{i=1,2}^{}2k_{1}\kappa_{op}\kappa _{ip} (I_{4_{i}}^{*}-1)\exp[k_{2}(I_{4_{i}}^{*}-1)^{2}-1]\\
\frac{\partial \Psi }{\partial I_{4_{i}}}&= \frac{k_{1}}{2k_{2}}2k_{2}(I_{4_{i}}^{*}-1)\frac{\partial I_{4_{i}}^{*}}{\partial I_{4_{i}}}\exp[k_{2}(I_{4_{i}}^{*}-1)^{2})-1]\\
&= 2k_{1}\kappa _{op}(1-2 \kappa _{ip})(I_{4_{i}}^{*}-1)\exp[k_{2}(I_{4_{i}}^{*}-1)^{2})-1].
\end{aligned}$$
We also need to calculate $\frac{\partial I_{4_{i}}^{*}}{\partial \mathbf C}$:
$$\begin{aligned}
\frac{\partial I_{4_{1}}^{*}}{\partial C}&= \frac{\partial I_{4_{1}}^{*}}{\partial I_{4_{1}}}\frac{\partial I_{4_{1}}}{\partial C}\\
&= 2 \kappa _{op}(1-2\kappa _{ip}) \mathbf m_{0}\otimes \mathbf m_{0}\\
\frac{\partial I_{4_{2}}^{*}}{\partial C}&= 2 \kappa _{op}(1-2\kappa _{ip}) \mathbf m_{0}'\otimes \mathbf m_{0}'
\end{aligned}$$
Then substituting these and previous values into the Cauchy stress tensor
$$\begin{aligned}
\mathbf \sigma &= 2 \mathbf F \left(\frac{p}{2} \mathbf C^{-1} \right)\mathbf F^{T}\\
&+2 \mathbf F \left(\frac{c}{2}+\sum_{i=1,2}^{}2k_{1}\kappa_{op}\kappa _{ip} (I_{4_{i}}^{*}-1)\exp[k_{2}(I_{4_{i}}^{*}-1)^{2}-1] \right) \mathbf F^{T}\\
&+2\mathbf F \cdot 2k_{1}\kappa _{op}(1-2 \kappa _{ip})(I_{4_{1}}^{*}-1)\exp[k_{2}(I_{4_{1}}^{*}-1)^{2})-1]2 \kappa _{op}(1-2\kappa _{ip}) \mathbf m_{0}\otimes \mathbf m_{0} \mathbf F^{T}\\
&+2\mathbf F \cdot 2k_{1}\kappa _{op}(1-2 \kappa _{ip})(I_{4_{2}}^{*}-1)\exp[k_{2}(I_{4_{2}}^{*}-1)^{2})-1]2 \kappa _{op}(1-2\kappa _{ip}) \mathbf m_{0}'\otimes \mathbf m_{0}' \mathbf F^{T}\\
\mathbf \sigma &= p \mathbf 1\\
&+ \left( c+4\sum_{i=1,2}^{}k_{1}\kappa_{op}\kappa _{ip} (I_{4_{i}}^{*}-1)\exp[k_{2}(I_{4_{i}}^{*}-1)^{2}-1]\right)\mathbf b\\
&+8k_{1}\kappa _{op}^{2}(1-2 \kappa _{ip})^{2}(I_{4_{1}}^{*}-1)\exp[k_{2}(I_{4_{1}}^{*}-1)^{2})-1] \mathbf m\otimes \mathbf m\\
&+8k_{1}\kappa _{op}^{2}(1-2 \kappa _{ip})^{2}(I_{4_{2}}^{*}-1)\exp[k_{2}(I_{4_{2}}^{*}-1)^{2})-1] \mathbf m'\otimes \mathbf m'
\end{aligned}$$
We still have 
$$\begin{aligned}
\mathbf b &= \begin{bmatrix}\lambda _{1}^{2} & 0 & 0\\
0 & \lambda _{2}^{2} & 0\\
0 & 0 & \frac{1}{(\lambda _{1}\lambda _{2})^{2}}\end{bmatrix}\\
\mathbf m \otimes \mathbf m&=  \begin{bmatrix}\lambda _{1}^{2}\cos ^{2}\theta  & \lambda _{1}\lambda _{2}\sin \theta \cos \theta  & 0\\
\lambda _{1}\lambda _{2}\sin \theta \cos \theta  & \lambda _{2}\sin ^{2}\theta  & 0\\
0 & 0 & 0\end{bmatrix}\\
\mathbf m' \otimes \mathbf m'&=  \begin{bmatrix}\lambda _{1}^{2}\cos ^{2}\theta  & -\lambda _{1}\lambda _{2}\sin^{2} \theta \cos \theta  & 0\\
-\lambda _{1}\lambda _{2}\sin \theta \cos \theta  & \lambda^{2} _{2}\sin ^{2}\theta  & 0\\
0 & 0 & 0\end{bmatrix}.
\end{aligned}$$
Since $I_{4_{1}}=I_{4_{2}}$,  $I_{4_{1}}^{*}=I_{4_{2}}^{*}=:I_{4}^{*}$  and 
$$\begin{aligned}
\mathbf \sigma &= p \mathbf 1 + \left(c + 8k_{1}\kappa _{op}\kappa _{ip}(I_{4}^{*}-1)\exp(\left[k_{2}(I_{4}^{*}-1)^{2}-1 \right]) \right)\mathbf b\\
&+8k_{1}\kappa _{op}^{2}(1-2 \kappa _{ip})^{2}(I_{4}^{*}-1)\exp[k_{2}(I_{4}^{*}-1)^{2})-1] \mathbf m\otimes \mathbf m\\
&+8k_{1}\kappa _{op}^{2}(1-2 \kappa _{ip})^{2}(I_{4}^{*}-1)\exp[k_{2}(I_{4}^{*}-1)^{2})-1] \mathbf m'\otimes \mathbf m'\\
\mathbf \sigma &= p \begin{bmatrix}1 & 0 & 0\\
0 & 1 & 0\\
0 & 0 & 1\end{bmatrix}\\
&+\left(c + 8k_{1}\kappa _{op}\kappa _{ip}(I_{4}^{*}-1)\exp(\left[k_{2}(I_{4}^{*}-1)^{2}-1 \right]) \right)\begin{bmatrix}\lambda _{1}^{2} & 0 & 0\\
0 & \lambda _{2}^{2} & 0\\
0 & 0 & \frac{1}{(\lambda _{1}\lambda _{2})^{2}}\end{bmatrix}\\
&+16k_{1}\kappa _{op}^{2}(1-2 \kappa _{ip})^{2}(I_{4}^{*}-1)\exp[k_{2}(I_{4}^{*}-1)^{2})-1]\begin{bmatrix}\lambda _{1}^{2}\cos ^{2}\theta  & 0  & 0\\
0  & \lambda _{2}^{2}\sin ^{2}\theta  & 0\\
0 & 0 & 0\end{bmatrix}.
\end{aligned}$$

Setting $\sigma _{33}=0$ gives
$$\begin{aligned}
\sigma _{33}&= 0\\
0&= p+\left( c+8k_{1}\kappa_{op}\kappa _{ip} (I_{4}^{*}-1)\exp[k_{2}(I_{4}^{*}-1)^{2}-1]\right) \frac{1}{(\lambda _{1}\lambda _{2})^{2}}\\
p &= -\frac{1}{(\lambda _{1}\lambda _{2})^{2}}\left( c+8k_{1}\kappa_{op}\kappa _{ip} (I_{4}^{*}-1)\exp[k_{2}(I_{4}^{*}-1)^{2}-1]\right)
\end{aligned}$$
Finally, the expressions for the stress are
$$\begin{aligned}
\sigma _{11}&= (c+8k_{1}\kappa_{op}\kappa _{ip} (I_{4}^{*}-1)\exp[k_{2}(I_{4}^{*}-1)^{2}-1]) \left(\lambda _{1}^{2}- \frac{1}{(\lambda _{1}\lambda _{2})^{2}} \right)\\
&+16k_{1}\kappa _{op}^{2}(1-2 \kappa _{ip})^{2}(I_{4}^{*}-1)\exp[k_{2}(I_{4}^{*}-1)^{2})-1]\lambda _{1}^{2}\cos ^{2}\theta \\
\sigma _{22}&= (c+8k_{1}\kappa_{op}\kappa _{ip} (I_{4}^{*}-1)\exp[k_{2}(I_{4}^{*}-1)^{2}-1]) \left(\lambda _{2}^{2}- \frac{1}{(\lambda _{1}\lambda _{2})^{2}} \right)\\
&+16k_{1}\kappa _{op}^{2}(1-2 \kappa _{ip})^{2}(I_{4}^{*}-1)\exp[k_{2}(I_{4}^{*}-1)^{2})-1]\lambda _{2}^{2}\sin ^{2}\theta 
\end{aligned}$$

$$I_{4}^{*}= 2 \kappa _{op}\kappa _{ip}I_{1}+2\kappa _{op}(1-2\kappa _{ip})I_{4}+(1-2\kappa _{op}-2\kappa _{op}\kappa _{ip})I_{n}$$

$$\begin{aligned}
I_{n}&= \mathbf m_{n}\cdot \mathbf m_{n}\\
&= \mathbf F \mathbf e_{3} \cdot \mathbf F \mathbf e_{3}\\
&= \begin{bmatrix}\lambda _{1} & 0 & 0 \\ 0 & \lambda _{2} & 0 \\ 0 & 0 & \frac{1}{(\lambda _{1}\lambda _{2})^{2}}\end{bmatrix}\begin{bmatrix}0 \\
0 \\
1\end{bmatrix} \cdot \begin{bmatrix}\lambda _{1} & 0 & 0 \\ 0 & \lambda _{2} & 0 \\ 0 & 0 & \frac{1}{(\lambda _{1}\lambda _{2})^{2}}\end{bmatrix}\begin{bmatrix}0 \\
0 \\
1\end{bmatrix}\\
&= \frac{1}{(\lambda _{1}\lambda _{2})^{4}}
\end{aligned}$$


![[Pasted image 20241025155246.png|700]]
