$$
\int_{k}^{k+1}\int_{-(x-k)}^{x-k}e^{y-x}dydx
$$

$$
\begin{align}
	\int_{0}^{1}\int_{-u}^{u}e^{y-u-k}dydu  & =\int_{0}^1 [e^{ y-u-k }]_{-u}^u du \\
 & =\int_{0}^1(e^{-k}-e^{-2u-k})du \\
 & =e^{-k}\left[ u+ \frac{1}{2}e^{ -2u } \right]_{0}^1 \\
 & =\frac{1}{2}e^{ -k }(1+e^{ -2 }).
\end{align}
$$

**Steps:**

**Step 1:** Let $\int_S e^{y-x} dS = \int_{S_0} e^{y-x} dS + \int_{S_1} e^{y-x} dS + \dots=\sum_{k=0}^\infty \int_{S_k} e^{y-x} dS$, where $S_k$ is the $k$-th triangle.

**Step 2:** Calculate $\int_{S_k} e^{y-x} dS$. $S_k$ is defined as $S_k=\{(x,y): k \leq x \leq k+1, -(x-k) \leq y \leq x-k\}$, so the integral over the $k$-th triangle is 

$$\int_{k}^{k+1}\int_{-(x-k)}^{x-k}e^{y-x}dydx.$$

**Step 3:** Substitute $u=x-k$ to simplify and compute the integral as

$$\begin{align}
	\int_{0}^{1}\int_{-u}^{u}e^{y-u-k}dydu  & =\int_{0}^1 [e^{ y-u-k }]_{-u}^u du \\
 & =\int_{0}^1(e^{-k}-e^{-2u-k})du \\
 & =e^{-k}\left[ u+ \frac{1}{2}e^{ -2u } \right]_{0}^1 \\
 & =\frac{1}{2}e^{ -k }(1+e^{ -2 }).
\end{align}$$

**Step 4:** Sum the geometric series
$$
\begin{align}
	\sum_{k=0}^\infty\frac{1}{2}e^{ -k }(1+e^{ -2 }) & = \frac{1+e^{ -2 }}{2}\sum_{k=0}^\infty e^{ -k } \\
 & =\frac{1+e^{ -2 }}{2(1-e^{ -1 })} \\
 & \approx 0.898
\end{align}
$$

....

**Final Answer:** 0.898
